changed P5

Projet_SAV_P3bis.v
@@ -1,6 +1,6 @@
 Add LoadPath "C:\Users\Hp\Documents\Coq" as CoqDirectory.
 Add LoadPath "/Users/samuel/Documents/Documents-L3/PolyCours/S2/Sem/projet_Semantique" as CoqDirectory.
-Load Projet_SAV_P2.
+Load Projet_SAV_Lemmas.
 
 
 
@@ -15,8 +15,8 @@ Inductive stack :=
     | empty_stack : stack
     | const_stack : (codeBloc * stack) -> stack -> stack.
 
-Notation "Grab ; tl " := (grab tl) (at level 20).
-Notation "Push c ; tl " := (push c tl) (at level 20).
+(*Notation "Grab ; tl " := (grab tl) (at level 20).
+Notation "Push c ; tl " := (push c tl) (at level 20).*)
 Notation " p # s " := (const_stack p s) (at level 19).
 
 
@@ -35,15 +35,15 @@ Definition transitionFunction : krivineState -> option krivineState :=
   fun ks => match ks return option krivineState with 
     | (Access 0, (c_0, e_0) # _, s) => Some (c_0, e_0, s)
     | (Access (S n), _ # tl, s)     => Some (Access n, tl, s)
-    | (Push c_2; c, e, s)           => Some (c, e, (c_2, e) # s)
-    | (Grab; c, e, t # s)           =>  Some (c, t # e, s)
+    | (push c_2 c, e, s)           => Some (c, e, (c_2, e) # s)
+    | (grab c, e, t # s)           =>  Some (c, t # e, s)
     | _ => None
 end.
 
 Fixpoint comp (t: lambdaTermeN) : codeBloc :=
   match t: lambdaTermeN return codeBloc with
     | var n => Access n
-    | lambda t_0 => Grab; comp t_0
+    | lambda t_0 => grab (comp t_0)
     | app t_0 t_1 => push (comp t_1) (comp t_0)
 end.
 
@@ -55,7 +55,7 @@ Fixpoint tau_code (code: codeBloc) : lambdaTermeN :=
   match code return lambdaTermeN with
     | Access n => var n
     | push c_2 c_1 => app (tau_code c_1) (tau_code c_2)
-    | Grab; c => lambda (tau_code c)
+    | grab c => lambda (tau_code c)
 end.
 
 Fixpoint tau_stack (s: stack) : list lambdaTermeN :=
@@ -106,56 +106,44 @@ Lemma comp_is_comp_glob: forall t: lambdaTermeN, tau (comp_glob t) = tau_code (c
 Proof.
   move => t.
   induction t.
-  simpl.
-  unfold tau_tuple.
-  simpl.
-  trivial.
-  simpl.
-  unfold tau_tuple.
-  simpl.
-  rewrite prop0.
-  trivial.
-  simpl.
-  unfold tau_tuple.
-  simpl.
-  rewrite prop0.
-  rewrite prop0.
-  trivial.
+  all : simpl.
+  all : unfold tau_tuple.
+  all : simpl.
+  2-3 : repeat rewrite prop0.
+  all : trivial.
 Qed.
 
 Lemma comp_and_tau: forall t: lambdaTermeN, tau (comp_glob t) = t.
 Proof.
-  induction t; simpl.
+  induction t.
+  all : simpl.
+  all : unfold tau_tuple.
+  all : simpl.
   trivial.
-  unfold tau_tuple.
-  simpl.
-  rewrite prop0.
-  rewrite <- comp_is_comp_glob.
+  all : repeat rewrite prop0.
+  all : repeat rewrite <- comp_is_comp_glob.
   rewrite IHt.
   trivial.
-  unfold tau_tuple.
-  simpl.
-  repeat rewrite prop0.
-  repeat (rewrite <- comp_is_comp_glob).
   rewrite IHt1 IHt2.
   trivial.
 Qed.
 
 Lemma grab_beta_red : forall c c1 : codeBloc, forall s s1 : stack,
-  List.Forall (fun t => C[0](t)) (tau_stack s) -> (app (tau_tuple (grab c) s) (tau_tuple c1 s1)) beta-> (tau_tuple c (element (c1, s1) s)).
+  List.Forall (fun t => C[0](t)) (tau_stack s) -> (app (tau_tuple (grab c) s) (tau_tuple c1 s1)) beta-> (tau_tuple c ((c1, s1) # s)).
 Proof.
   move => c c1 s s1 Hl.
   unfold tau_tuple.
   simpl.
   suff: List.map incr_free (tau_stack s) = tau_stack s.
-  intro H.
-  rewrite H.
-  suff : ((tau_code c) [0 <-- (tau_code c1) [0 <-- tau_stack s1] :: tau_stack s]) = (tau_code c) [1 <-- tau_stack s] [0 <- (tau_code c1) [0 <-- tau_stack s1]].
-  intro H0; rewrite H0.
-  apply (evaluation (tau_code c) [1 <-- tau_stack s] (tau_code c1) [0 <-- tau_stack s1]).
+  + intro H.
+    rewrite H.
+    suff : ((tau_code c) [0 <-- (tau_code c1) [0 <-- tau_stack s1] :: tau_stack s])
+        = (tau_code c) [1 <-- tau_stack s] [0 <- (tau_code c1) [0 <-- tau_stack s1]].
+      intro H0; rewrite H0.
+    apply (evaluation (tau_code c) [1 <-- tau_stack s] (tau_code c1) [0 <-- tau_stack s1]).
 
-  apply prop2.
-  simpl.
-  trivial.
-  apply lemma23; trivial.
+    apply prop2.
+    simpl.
+    trivial.
+  + apply lemma23; trivial.
 Qed.
